Core.thy
@@ -4,11 +4,11 @@ begin
 
 definition ite:: "bool \<Rightarrow> 's \<Rightarrow> 's \<Rightarrow> 's" where "ite a B C  \<equiv> if a then B else C"
 
-lemma ite_true[simp]: "(ite a B C) \<and> a \<Longrightarrow> B"
+lemma ite_true[simp]: "(ite True B C) \<Longrightarrow> B"
   apply(simp add: ite_def)
   done
 
-lemma ite_false[simp]: "(ite a B C) \<and> \<not> a \<Longrightarrow> C"
+lemma ite_false[simp]: "(ite False B C) \<Longrightarrow> C"
   apply(simp add: ite_def)
   done
 
